@prefix flow: <http://example.org/flowmetrics#> .
@prefix rdfs: <http://www.w3.org/2000/01/rdf-schema#> .
@prefix skos: <http://www.w3.org/2004/02/skos/core#> .
@prefix xsd: <http://www.w3.org/2001/XMLSchema#> .

@prefix rdf: <http://www.w3.org/1999/02/22-rdf-syntax-ns#> .
@prefix cso: <http://cso.kmi.open.ac.uk/schema/cso#> .
@prefix owl: <http://www.w3.org/2002/07/owl#> .
@prefix sh: <http://www.w3.org/ns/shacl#> .


#################################################################
#    Annotation properties
#################################################################

###  http://example.org/flowmetrics#hasEngagementImpact
flow:hasEngagementImpact rdf:type owl:AnnotationProperty ;
    rdfs:label "hasEngagementImpact"@en ;    # Human-readable label
    rdfs:comment "Defines the Engagement impact as one of the five semantic stages of impact."@en ; # Description
    rdfs:domain flow:TopicPair ;      
    rdfs:range skos:Concept .  


###  http://example.org/flowmetrics#hasFeedbackImpact
flow:hasFeedbackImpact rdf:type owl:AnnotationProperty ;
    rdfs:label "hasFeedbackImpact"@en ;    # Human-readable label
    rdfs:comment "Defines the Feedback impact as one of the five semantic stages of impact."@en ; # Description
    rdfs:domain flow:TopicPair .


###  http://example.org/flowmetrics#hasInfluenceImpact
flow:hasInfluenceImpact rdf:type owl:AnnotationProperty ;
    rdfs:label "hasInfluenceImpact"@en ;    # Human-readable label
    rdfs:comment "Defines the Influence impact as one of the five semantic stages of impact."@en ; # Description
    rdfs:domain flow:TopicPair .


###  http://example.org/flowmetrics#hasOutcomeImpact
flow:hasOutcomeImpact rdf:type owl:AnnotationProperty ;
    rdfs:label "hasOutcomeImpact"@en ;    # Human-readable label
    rdfs:comment "Defines the Outcome impact as one of the five semantic stages of impact."@en ; # Description
    rdfs:domain flow:TopicPair .


###  http://example.org/flowmetrics#hasReachImpact
flow:hasReachImpact rdf:type owl:AnnotationProperty ;
    rdfs:label "hasReachImpact"@en ;    # Human-readable label
    rdfs:comment "Defines the Reach impact as one of the five semantic stages of impact."@en ; # Description
    rdfs:domain flow:TopicPair .


###  http://example.org/flowmetrics#hasSharedConcept
flow:hasSharedConcept rdf:type owl:AnnotationProperty ;
    rdfs:label "hasSharedConcept"@en ;    # Human-readable label
    rdfs:comment "The shared concept between two nodes. This is associted to the topic pair rather than the single individual node."@en ; # Description
    rdfs:domain flow:TopicPair ;      
    rdfs:range rdfs:Literal .  


###  http://example.org/flowmetrics#hasTopic
flow:hasTopic rdf:type owl:AnnotationProperty ;
            rdfs:range flow:ResearchTopic ;
            rdfs:domain flow:TopicPair ;
            rdfs:label "hasTopic"@en ;    # Human-readable label
            rdfs:comment "This relationship defines the topic nodes of an edge (topic pair)."@en . # Description


###  http://example.org/flowmetrics#platform
flow:platform rdf:type owl:AnnotationProperty ;
    rdfs:label "platform"@en ;    # Human-readable label
    rdfs:comment "The platform name providing the metric."@en ; # Description
    rdfs:domain flow:TopicPair .


###  http://example.org/flowmetrics#score
flow:score rdf:type owl:AnnotationProperty ;
    rdfs:label "score"@en ;    # Human-readable label
    rdfs:comment "The score associated to a given platform."@en ; # Description
    rdfs:domain flow:TopicPair .

#################################################################
#    Classes
#################################################################

###  http://example.org/flowmetrics#Topic
flow:ResearchTopic rdf:type owl:Class ;
       owl:sameAs skos:Concept ;
       owl:sameAs cso:Topic .

###  http://example.org/flowmetrics#TopicPair
flow:TopicPair rdf:type owl:Class ;
        sh:property [                 
            sh:path flow:hasTopic ;           # constrains the values of flow:hasTopic
            sh:maxCount 2 ;
            sh:minCount 2 ; 
            sh:node flow:ResearchTopic 
        ] .

